DY/Bytes/Invariants.lean
@@ -4,39 +4,37 @@ import DY.Trace
 
 namespace DY
 
-variable {CtorId: Type}
-variable [BytesCtors CtorId]
+variable [BytesFunctor]
 
 -- Well formed
 
 def BytesWellFormedT := ProofTrace → Prop
-def BytesWellFormedT.default: BytesWellFormedT := fun _ => False
 
 class BytesWellFormed where
-  funs: BytesFunCtors BytesWellFormedT
+  funs: Bytes.Function BytesWellFormedT
 
 def Bytes.WellFormed [BytesWellFormed] (b: Bytes) : BytesWellFormedT :=
-  Bytes.mkRec BytesWellFormed.funs .default b
+  Bytes.rec BytesWellFormed.funs b
 
-class HasBytesWellFormed [BytesWellFormed] (id: CtorId) {ctor: BytesCtor} [ctor.HasCtorAt id] (binv: outParam (BytesFunCtor id BytesWellFormedT)) where
-  pf: BytesWellFormed.funs id = binv.into
+class HasBytesWellFormed [BytesWellFormed] {SubF: Type → Type} [SubBytesFunctor SubF] [BytesFunctor.Has SubF] (binv: outParam (Bytes.PartialFunction SubF BytesWellFormedT)) where
+  pf: Bytes.SubFunction binv BytesWellFormed.funs
   dummy: Unit -- leanprover/lean4#11477 workaround
 
+@[simp]
 theorem Bytes.WellFormed.eq
-  [tc_binv: BytesWellFormed]
-  (id: CtorId) {ctor: BytesCtor} [ctor.HasCtorAt id]
-  {binv: BytesFunCtor id BytesWellFormedT}
-  [tc: HasBytesWellFormed id binv]
-  (b: BytesView id)
+  {SubF: Type → Type} [SubBytesFunctor SubF] [BytesFunctor.Has SubF]
+  [BytesWellFormed]
+  {binv: Bytes.PartialFunction SubF BytesWellFormedT}
+  [tc: HasBytesWellFormed binv]
+  (b: BytesView SubF)
   (tr: ProofTrace)
-  : Bytes.WellFormed (b.pack) tr = binv.func b.data b.dataBytes Bytes.WellFormed tr
+  : b.pack.WellFormed tr = binv b (fun y _ => Bytes.WellFormed y) tr
   := by
-    have lem {a b} (f g: a → b) (x: a): f = g → f x = g x := by grind
-    apply lem
-    apply Bytes.mkRec.eqView
-    exact tc.pf
+    apply congrFun
+    have := tc.pf
+    apply Bytes.rec_eq
 
-grind_pattern Bytes.WellFormed.eq => Bytes.WellFormed (b.pack) tr
+grind_pattern Bytes.WellFormed.eq => b.pack.WellFormed tr
 
 -- Well formed later
 
@@ -44,7 +42,7 @@ def BytesWellFormedLaterT (bwf: BytesWellFormedT) :=
   ∀ tr1 tr2, tr1 ≤ tr2 → bwf tr1 → bwf tr2
 
 class BytesWellFormedLater [BytesWellFormed] where
-  proofs: BytesFunCtorsProof1 BytesWellFormed.funs BytesWellFormedT.default BytesWellFormedLaterT
+  proofs: Bytes.Proof1 BytesWellFormed.funs BytesWellFormedLaterT
 
 theorem Bytes.WellFormed.later
   [BytesWellFormed] [BytesWellFormedLater]
@@ -72,34 +70,32 @@ def Usage.nothing: Usage where
   data := none
 
 def GetUsageT := ProofTrace → Usage
-def GetUsageT.default: GetUsageT := fun _ => Usage.nothing
 
 class GetUsage where
-  funs: BytesFunCtors GetUsageT
+  funs: Bytes.Function GetUsageT
 
-noncomputable
 def Bytes.usage [GetUsage] (b: Bytes) : GetUsageT :=
-  Bytes.mkRec GetUsage.funs .default b
+  Bytes.rec GetUsage.funs b
 
-class HasGetUsage [GetUsage] (id: CtorId) {ctor: BytesCtor} [ctor.HasCtorAt id] (binv: outParam (BytesFunCtor id GetUsageT)) where
-  pf: GetUsage.funs id = binv.into
+class HasGetUsage [GetUsage] {SubF: Type → Type} [SubBytesFunctor SubF] [BytesFunctor.Has SubF] (binv: outParam (Bytes.PartialFunction SubF GetUsageT)) where
+  pf: Bytes.SubFunction binv GetUsage.funs
   dummy: Unit -- leanprover/lean4#11477 workaround
 
+@[simp]
 theorem Bytes.usage.eq
-  [tc_binv: GetUsage]
-  (id: CtorId) {ctor: BytesCtor} [ctor.HasCtorAt id]
-  {binv: BytesFunCtor id GetUsageT}
-  [tc: HasGetUsage id binv]
-  (b: BytesView id)
+  {SubF: Type → Type} [SubBytesFunctor SubF] [BytesFunctor.Has SubF]
+  [GetUsage]
+  {binv: Bytes.PartialFunction SubF GetUsageT}
+  [tc: HasGetUsage binv]
+  (b: BytesView SubF)
   (tr: ProofTrace)
-  : Bytes.usage (b.pack) tr = binv.func b.data b.dataBytes Bytes.usage tr
+  : b.pack.usage tr = binv b (fun y _ => Bytes.usage y) tr
   := by
-    have lem {a b} (f g: a → b) (x: a): f = g → f x = g x := by grind
-    apply lem
-    apply Bytes.mkRec.eqView
-    exact tc.pf
+    apply congrFun
+    have := tc.pf
+    apply Bytes.rec_eq
 
-grind_pattern Bytes.usage.eq => Bytes.usage (b.pack) tr
+grind_pattern Bytes.usage.eq => (b.pack).usage tr
 
 -- Usage later
 
@@ -108,7 +104,7 @@ def GetUsageLaterT (x: BytesWellFormedT × GetUsageT) :=
   ∀ tr1 tr2: ProofTrace, tr1 ≤ tr2 → wf tr1 → usg tr1 = usg tr2
 
 class GetUsageLater [BytesWellFormed] [GetUsage] where
-  proofs: BytesFunCtorsProof2 BytesWellFormed.funs GetUsage.funs BytesWellFormedT.default GetUsageT.default GetUsageLaterT
+  proofs: Bytes.Proof2 BytesWellFormed.funs GetUsage.funs GetUsageLaterT
 
 theorem Bytes.usage_later
   [BytesWellFormed] [GetUsage] [GetUsageLater]
@@ -126,34 +122,31 @@ grind_pattern Bytes.usage_later => Bytes.usage b tr1, tr1 ≤ tr2
 -- Label
 
 def GetLabelT := ProofTrace → Label
-def GetLabelT.default: GetLabelT := fun _ => Label.secret
 
 class GetLabel where
-  funs: BytesFunCtors GetLabelT
+  funs: Bytes.Function GetLabelT
 
-noncomputable
 def Bytes.label [GetLabel] (b: Bytes) : GetLabelT :=
-  Bytes.mkRec GetLabel.funs .default b
+  Bytes.rec GetLabel.funs b
 
-class HasGetLabel [GetLabel] (id: CtorId) {ctor: BytesCtor} [ctor.HasCtorAt id] (binv: outParam (BytesFunCtor id GetLabelT)) where
-  pf: GetLabel.funs id = binv.into
+class HasGetLabel [GetLabel] {SubF: Type → Type} [SubBytesFunctor SubF] [BytesFunctor.Has SubF] (binv: outParam (Bytes.PartialFunction SubF GetLabelT)) where
+  pf: Bytes.SubFunction binv GetLabel.funs
   dummy: Unit -- leanprover/lean4#11477 workaround
 
 theorem Bytes.label.eq
-  [tc_binv: GetLabel]
-  (id: CtorId) {ctor: BytesCtor} [ctor.HasCtorAt id]
-  {binv: BytesFunCtor id GetLabelT}
-  [tc: HasGetLabel id binv]
-  (b: BytesView id)
+  {SubF: Type → Type} [SubBytesFunctor SubF] [BytesFunctor.Has SubF]
+  [GetLabel]
+  {binv: Bytes.PartialFunction SubF GetLabelT}
+  [tc: HasGetLabel binv]
+  (b: BytesView SubF)
   (tr: ProofTrace)
-  : Bytes.label (b.pack) tr = binv.func b.data b.dataBytes Bytes.label tr
+  : b.pack.label tr = binv b (fun y _ => Bytes.label y) tr
   := by
-    have lem {a b} (f g: a → b) (x: a): f = g → f x = g x := by grind
-    apply lem
-    apply Bytes.mkRec.eqView
-    exact tc.pf
+    apply congrFun
+    have := tc.pf
+    apply Bytes.rec_eq
 
-grind_pattern Bytes.label.eq => Bytes.label (b.pack) tr
+grind_pattern Bytes.label.eq => b.pack.label tr
 
 -- Label later
 
@@ -162,7 +155,7 @@ def GetLabelLaterT (x: BytesWellFormedT × GetLabelT) :=
   ∀ tr1 tr2: ProofTrace, tr1 ≤ tr2 → wf tr1 → usg tr1 = usg tr2
 
 class GetLabelLater [BytesWellFormed] [GetLabel] where
-  proofs: BytesFunCtorsProof2 BytesWellFormed.funs GetLabel.funs BytesWellFormedT.default GetLabelT.default GetLabelLaterT
+  proofs: Bytes.Proof2 BytesWellFormed.funs GetLabel.funs GetLabelLaterT
 
 theorem Bytes.label_later
   [BytesWellFormed] [GetLabel] [GetLabelLater]
@@ -181,31 +174,28 @@ grind_pattern Bytes.label_later => Bytes.label b tr1, tr1 ≤ tr2
 
 def BytesInvariantT := ProofTrace → Prop
 
-def BytesInvariantT.default: BytesInvariantT := fun _ => False
-
 class BytesInvariant where
-  funs: BytesFunCtors BytesInvariantT
+  funs: Bytes.Function BytesInvariantT
 
 def Bytes.Invariant [BytesInvariant] (b: Bytes) (tr: ProofTrace) : Prop :=
-  Bytes.mkRec BytesInvariant.funs .default b tr
+  Bytes.rec BytesInvariant.funs b tr
 
-class HasBytesInvariant [BytesInvariant] (id: CtorId) {ctor: BytesCtor} [ctor.HasCtorAt id] (binv: outParam (BytesFunCtor id BytesInvariantT)) where
-  pf: BytesInvariant.funs id = binv.into
+class HasBytesInvariant [BytesInvariant] {SubF: Type → Type} [SubBytesFunctor SubF] [BytesFunctor.Has SubF] (binv: outParam (Bytes.PartialFunction SubF BytesInvariantT)) where
+  pf: Bytes.SubFunction binv BytesInvariant.funs
   dummy: Unit -- leanprover/lean4#11477 workaround
 
 theorem Bytes.Invariant.eq
-  [tc_binv: BytesInvariant]
-  (id: CtorId) {ctor: BytesCtor} [ctor.HasCtorAt id]
-  {binv: BytesFunCtor id BytesInvariantT}
-  [tc: HasBytesInvariant id binv]
-  (b: BytesView id)
+  {SubF: Type → Type} [SubBytesFunctor SubF] [BytesFunctor.Has SubF]
+  [BytesInvariant]
+  {binv: Bytes.PartialFunction SubF BytesInvariantT}
+  [tc: HasBytesInvariant binv]
+  (b: BytesView SubF)
   (tr: ProofTrace)
-  : Bytes.Invariant (b.pack) tr = binv.func b.data b.dataBytes Bytes.Invariant tr
+  : b.pack.Invariant tr = binv b (fun y _ => Bytes.Invariant y) tr
   := by
-    have lem {a b} (f g: a → b) (x: a): f = g → f x = g x := by grind
-    apply lem
-    apply Bytes.mkRec.eqView
-    exact tc.pf
+    apply congrFun
+    have := tc.pf
+    apply Bytes.rec_eq
 
 grind_pattern Bytes.Invariant.eq => Bytes.Invariant (b.pack) tr
 
@@ -216,7 +206,7 @@ def BytesInvariantImpliesBytesWellFormedT (x: BytesInvariantT × BytesWellFormed
   ∀ tr, binv tr → bwf tr
 
 class BytesInvariantImpliesBytesWellFormed [BytesWellFormed] [BytesInvariant] where
-  proofs: BytesFunCtorsProof2 BytesInvariant.funs BytesWellFormed.funs BytesInvariantT.default BytesWellFormedT.default BytesInvariantImpliesBytesWellFormedT
+  proofs: Bytes.Proof2 BytesInvariant.funs BytesWellFormed.funs BytesInvariantImpliesBytesWellFormedT
 
 theorem Bytes.Invariant_implies_WellFormed
   [BytesWellFormed] [BytesInvariant] [BytesInvariantImpliesBytesWellFormed]
@@ -236,7 +226,7 @@ def BytesInvariantLaterT (binv: BytesInvariantT) :=
   ∀ tr1 tr2, tr1 ≤ tr2 → binv tr1 → binv tr2
 
 class BytesInvariantLater [BytesInvariant] where
-  proofs: BytesFunCtorsProof1 BytesInvariant.funs BytesInvariantT.default BytesInvariantLaterT
+  proofs: Bytes.Proof1 BytesInvariant.funs BytesInvariantLaterT
 
 theorem Bytes.Invariant.later
   [BytesInvariant] [BytesInvariantLater]
@@ -251,94 +241,173 @@ theorem Bytes.Invariant.later
 
 grind_pattern Bytes.Invariant.later => Bytes.Invariant b tr1, tr1 ≤ tr2
 
-structure BytesCtorInvariants.Internal (ctor: BytesCtor) where
-  well_formed: BytesFunCtor.Internal ctor BytesWellFormedT
-  well_formed_later: [BytesWellFormed] → BytesFunCtorProof1.Internal Bytes.WellFormed well_formed BytesWellFormedLaterT
+structure Bytes.PartialInvariants (SubF: Type → Type) [SubBytesFunctor SubF] where
+  well_formed: Bytes.PartialFunction SubF BytesWellFormedT
+  well_formed_later: [BytesWellFormed] → Bytes.PartialProof1 well_formed Bytes.WellFormed BytesWellFormedLaterT
+  := by
+    intro _ x rec tr1 tr2
+    cases x
+    simp_all [DY.ALaCarte.FunctorSizeOf.sizeOf, BytesWellFormedLaterT] <;> grind
 
-  usage: BytesFunCtor.Internal ctor GetUsageT
-  usage_later: [BytesWellFormed] → [GetUsage] → BytesFunCtorProof2.Internal Bytes.WellFormed Bytes.usage well_formed usage GetUsageLaterT
+  usage: Bytes.PartialFunction SubF GetUsageT
+  usage_later: [BytesWellFormed] → [GetUsage] → Bytes.PartialProof2 well_formed usage Bytes.WellFormed Bytes.usage GetUsageLaterT
+  := by
+    intro _ _ x rec tr1 tr2
+    cases x
+    simp_all [DY.ALaCarte.FunctorSizeOf.sizeOf, GetUsageLaterT] <;> grind
 
-  label: [GetUsage] → BytesFunCtor.Internal ctor GetLabelT
-  label_later: [BytesWellFormed] → [GetUsage] → [GetUsageLater] → [GetLabel] → BytesFunCtorProof2.Internal Bytes.WellFormed Bytes.label well_formed label GetLabelLaterT
+  label: [GetUsage] → Bytes.PartialFunction SubF GetLabelT
+  label_later: [BytesWellFormed] → [GetUsage] → [GetUsageLater] → [GetLabel] → Bytes.PartialProof2 well_formed label Bytes.WellFormed Bytes.label GetLabelLaterT
+  := by
+    intro _ _ _ _ x rec tr1 tr2
+    cases x
+    simp_all [DY.ALaCarte.FunctorSizeOf.sizeOf, GetLabelLaterT] <;> grind
 
-  invariant: [BytesWellFormed] → [GetUsage] → [GetLabel] → BytesFunCtor.Internal ctor BytesInvariantT
-  invariant_implies_wellformed: [BytesWellFormed] → [GetUsage] → [GetLabel] → [BytesInvariant] → BytesFunCtorProof2.Internal Bytes.Invariant Bytes.WellFormed invariant well_formed BytesInvariantImpliesBytesWellFormedT
-  invariant_later: [BytesWellFormed] → [BytesWellFormedLater] → [GetUsage] → [GetUsageLater] → [GetLabel] → [GetLabelLater] → [BytesInvariant] → [BytesInvariantImpliesBytesWellFormed] → BytesFunCtorProof1.Internal Bytes.Invariant invariant BytesInvariantLaterT
-  -- ...
+  invariant: [BytesWellFormed] → [GetUsage] → [GetLabel] → Bytes.PartialFunction SubF BytesInvariantT
+  invariant_implies_wellformed: [BytesWellFormed] → [GetUsage] → [GetLabel] → [BytesInvariant] → Bytes.PartialProof2 invariant well_formed Bytes.Invariant Bytes.WellFormed BytesInvariantImpliesBytesWellFormedT
+  := by
+    intro _ _ _ _ x rec tr
+    cases x
+    simp_all [DY.ALaCarte.FunctorSizeOf.sizeOf, BytesInvariantImpliesBytesWellFormedT] <;> grind
+  invariant_later: [BytesWellFormed] → [BytesWellFormedLater] → [GetUsage] → [GetUsageLater] → [GetLabel] → [GetLabelLater] → [BytesInvariant] → [BytesInvariantImpliesBytesWellFormed] → Bytes.PartialProof1 invariant Bytes.Invariant BytesInvariantLaterT
+  := by
+    intro _ _ _ _ _ _ _ _ x rec tr1 tr2
+    cases x
+    simp_all [DY.ALaCarte.FunctorSizeOf.sizeOf, BytesInvariantLaterT] <;> grind
 
-def BytesCtorInvariants.ById (id: CtorId) := BytesCtorInvariants.Internal (BytesCtors.ctors id)
-def BytesCtorInvariants (id: CtorId) {ctor: BytesCtor} [ctor.HasCtorAt id] := BytesCtorInvariants.Internal ctor
+class BytesInvariants where
+  invs: Bytes.PartialInvariants BytesF
 
-def BytesCtorInvariants.into
-  {id: CtorId} {ctor: BytesCtor} [ctor.HasCtorAt id]
-  (f: BytesCtorInvariants id)
-  : BytesCtorInvariants.ById id
+instance [BytesInvariants]: BytesWellFormed where
+  funs := BytesInvariants.invs.well_formed
+
+instance [BytesInvariants]: BytesWellFormedLater where
+  proofs := BytesInvariants.invs.well_formed_later
+
+instance [BytesInvariants]: GetUsage where
+  funs := BytesInvariants.invs.usage
+
+instance [BytesInvariants]: GetUsageLater where
+  proofs := BytesInvariants.invs.usage_later
+
+instance [BytesInvariants]: GetLabel where
+  funs := BytesInvariants.invs.label
+
+instance [BytesInvariants]: GetLabelLater where
+  proofs := BytesInvariants.invs.label_later
+
+instance [BytesInvariants]: BytesInvariant where
+  funs := BytesInvariants.invs.invariant
+
+instance [BytesInvariants]: BytesInvariantImpliesBytesWellFormed where
+  proofs := BytesInvariants.invs.invariant_implies_wellformed
+
+instance [BytesInvariants]: BytesInvariantLater where
+  proofs := BytesInvariants.invs.invariant_later
+
+class BytesInvariants.HasStep
+  [BytesInvariants]
+  {SubF1 SubF2: Type → Type}
+  [SubBytesFunctor SubF1] [SubBytesFunctor SubF2]
+  [BytesFunctor.HasStep SubF1 SubF2]
+  (partialInvs1: outParam (Bytes.PartialInvariants SubF1))
+  (partialInvs2: Bytes.PartialInvariants SubF2)
   where
-    well_formed := BytesFunCtor.into f.well_formed
-    well_formed_later := BytesFunCtorProof1.into f.well_formed_later
+    [well_formed_sub: Bytes.SubFunctionStep partialInvs1.well_formed partialInvs2.well_formed]
+    [usage_sub: Bytes.SubFunctionStep partialInvs1.usage partialInvs2.usage]
+    [label_sub: Bytes.SubFunctionStep partialInvs1.label partialInvs2.label]
+    [invariant_sub: Bytes.SubFunctionStep partialInvs1.invariant partialInvs2.invariant]
 
-    usage := BytesFunCtor.into f.usage
-    usage_later := BytesFunCtorProof2.into f.usage_later
+class BytesInvariants.Has
+  [BytesInvariants]
+  {SubF: Type → Type}
+  [SubBytesFunctor SubF]
+  [BytesFunctor.Has SubF]
+  (partialInvs: outParam (Bytes.PartialInvariants SubF))
+  where
+    [well_formed_sub: Bytes.SubFunction partialInvs.well_formed BytesWellFormed.funs]
+    [usage_sub: Bytes.SubFunction partialInvs.usage GetUsage.funs]
+    [label_sub: Bytes.SubFunction partialInvs.label GetLabel.funs]
+    [invariant_sub: Bytes.SubFunction partialInvs.invariant BytesInvariant.funs]
 
-    label := BytesFunCtor.into f.label
-    label_later := BytesFunCtorProof2.into f.label_later
+namespace BytesInvariants
 
-    invariant := BytesFunCtor.into f.invariant
-    invariant_implies_wellformed := BytesFunCtorProof2.into f.invariant_implies_wellformed
-    invariant_later := BytesFunCtorProof1.into f.invariant_later
+instance [BytesInvariants]: BytesInvariants.Has (BytesInvariants.invs) where
 
+instance
+  [BytesInvariants]
+  {SubF1 SubF2: Type → Type}
+  [SubBytesFunctor SubF1] [SubBytesFunctor SubF2]
+  [BytesFunctor.HasStep SubF1 SubF2]
+  [BytesFunctor.Has SubF2]
+  (partialInvs1: Bytes.PartialInvariants SubF1)
+  (partialInvs2: Bytes.PartialInvariants SubF2)
+  [inst1: BytesInvariants.HasStep partialInvs1 partialInvs2]
+  [inst2: BytesInvariants.Has partialInvs2]
+  : BytesInvariants.Has partialInvs1
+  := by
+    cases inst1
+    cases inst2
+    exact {}
 
-class BytesCtorsInvariants where
-  funs: (id: CtorId) → BytesCtorInvariants.ById id
+end BytesInvariants
 
-instance [BytesCtorsInvariants]: BytesWellFormed where
-  funs id := (BytesCtorsInvariants.funs id).well_formed
+def Bytes.PartialInvariants.combine
+  {t: Type} [DecidableEq t] [Ord t] [Std.LawfulEqOrd t] [Std.TransOrd t]
+  {SubFs: t → Type → Type} [∀ id, SubBytesFunctor (SubFs id)]
+  (invs: ∀ id, Bytes.PartialInvariants (SubFs id))
+  : Bytes.PartialInvariants (BytesFunctor.combine SubFs)
+  where
+    well_formed := Bytes.PartialFunction.combine (fun id => (invs id).well_formed)
+    well_formed_later := Bytes.PartialProof1.combine (fun id => (invs id).well_formed_later)
 
-instance [BytesCtorsInvariants]: BytesWellFormedLater where
-  proofs id := (BytesCtorsInvariants.funs id).well_formed_later
+    usage := Bytes.PartialFunction.combine (fun id => (invs id).usage)
+    usage_later := Bytes.PartialProof2.combine (fun id => (invs id).usage_later)
 
-instance [BytesCtorsInvariants]: GetUsage where
-  funs id := (BytesCtorsInvariants.funs id).usage
+    label := Bytes.PartialFunction.combine (fun id => (invs id).label)
+    label_later := Bytes.PartialProof2.combine (fun id => (invs id).label_later)
 
-instance [BytesCtorsInvariants]: GetUsageLater where
-  proofs id := (BytesCtorsInvariants.funs id).usage_later
+    invariant := Bytes.PartialFunction.combine (fun id => (invs id).invariant)
+    invariant_implies_wellformed := Bytes.PartialProof2.combine (fun id => (invs id).invariant_implies_wellformed)
+    invariant_later := Bytes.PartialProof1.combine (fun id => (invs id).invariant_later)
 
-instance [BytesCtorsInvariants]: GetLabel where
-  funs id := (BytesCtorsInvariants.funs id).label
+instance
+  [BytesInvariants]
+  {t: Type} [DecidableEq t] [Ord t] [Std.LawfulEqOrd t] [Std.TransOrd t]
+  (SubFs: t → Type → Type) [∀ id, SubBytesFunctor (SubFs id)]
+  (invs: ∀ id, Bytes.PartialInvariants (SubFs id))
+  (id: t)
+  : BytesInvariants.HasStep (invs id) (Bytes.PartialInvariants.combine invs)
+  :=
+    let wfs := (fun id => (invs id).well_formed)
+    let usages := (fun id => (invs id).usage)
+    let labels := (fun id => (invs id).label)
+    let invariants := (fun id => (invs id).invariant)
+    {
+      well_formed_sub := inferInstanceAs (Bytes.SubFunctionStep (wfs id) (Bytes.PartialFunction.combine wfs))
+      usage_sub := inferInstanceAs (Bytes.SubFunctionStep (usages id) (Bytes.PartialFunction.combine usages))
+      label_sub := inferInstanceAs (Bytes.SubFunctionStep (labels id) (Bytes.PartialFunction.combine labels))
+      invariant_sub := inferInstanceAs (Bytes.SubFunctionStep (invariants id) (Bytes.PartialFunction.combine invariants))
+    }
 
-instance [BytesCtorsInvariants]: GetLabelLater where
-  proofs id := (BytesCtorsInvariants.funs id).label_later
-
-instance [BytesCtorsInvariants]: BytesInvariant where
-  funs id := (BytesCtorsInvariants.funs id).invariant
-
-instance [BytesCtorsInvariants]: BytesInvariantImpliesBytesWellFormed where
-  proofs id := (BytesCtorsInvariants.funs id).invariant_implies_wellformed
-
-instance [BytesCtorsInvariants]: BytesInvariantLater where
-  proofs id := (BytesCtorsInvariants.funs id).invariant_later
-
-class HasBytesInvariants [BytesCtorsInvariants] (id: CtorId) {ctor: BytesCtor} [ctor.HasCtorAt id] (funs: outParam (BytesCtorInvariants id)) where
-  pf: BytesCtorsInvariants.funs id = funs.into
-
-instance [BytesCtorsInvariants] (id: CtorId) {ctor: BytesCtor} [ctor.HasCtorAt id] (funs: BytesCtorInvariants id) [tc: HasBytesInvariants id funs]: HasBytesWellFormed id funs.well_formed where
-  pf := by simp only [BytesWellFormed.funs, tc.pf, BytesCtorInvariants.into]
+instance [BytesInvariants] {SubF: Type → Type} [SubBytesFunctor SubF] [BytesFunctor.Has SubF] (invs: Bytes.PartialInvariants SubF) [tc: BytesInvariants.Has invs]: HasBytesWellFormed invs.well_formed where
+  pf := tc.well_formed_sub
   dummy := ()
 
-instance [BytesCtorsInvariants] (id: CtorId) {ctor: BytesCtor} [ctor.HasCtorAt id] (funs: BytesCtorInvariants id) [tc: HasBytesInvariants id funs]: HasGetUsage id funs.usage where
-  pf := by simp only [GetUsage.funs, tc.pf, BytesCtorInvariants.into]
+instance [BytesInvariants] {SubF: Type → Type} [SubBytesFunctor SubF] [BytesFunctor.Has SubF] (invs: Bytes.PartialInvariants SubF) [tc: BytesInvariants.Has invs]: HasGetUsage invs.usage where
+  pf := tc.usage_sub
   dummy := ()
 
-instance [BytesCtorsInvariants] (id: CtorId) {ctor: BytesCtor} [ctor.HasCtorAt id] (funs: BytesCtorInvariants id) [tc: HasBytesInvariants id funs]: HasGetLabel id funs.label where
-  pf := by simp only [GetLabel.funs, tc.pf, BytesCtorInvariants.into]
+instance [BytesInvariants] {SubF: Type → Type} [SubBytesFunctor SubF] [BytesFunctor.Has SubF] (invs: Bytes.PartialInvariants SubF) [tc: BytesInvariants.Has invs]: HasGetLabel invs.label where
+  pf := tc.label_sub
   dummy := ()
 
-instance [BytesCtorsInvariants] (id: CtorId) {ctor: BytesCtor} [ctor.HasCtorAt id] (funs: BytesCtorInvariants id) [tc: HasBytesInvariants id funs]: HasBytesInvariant id funs.invariant where
-  pf := by simp only [BytesInvariant.funs, tc.pf, BytesCtorInvariants.into]
+instance [BytesInvariants] {SubF: Type → Type} [SubBytesFunctor SubF] [BytesFunctor.Has SubF] (invs: Bytes.PartialInvariants SubF) [tc: BytesInvariants.Has invs]: HasBytesInvariant invs.invariant where
+  pf := tc.invariant_sub
   dummy := ()
 
 @[grind]
-def Bytes.Publishable [BytesCtorsInvariants] (b: Bytes) (tr: ProofTrace) :=
+def Bytes.Publishable [BytesInvariants] (b: Bytes) (tr: ProofTrace) :=
   b.Invariant tr ∧
   (b.label tr).canFlow Label.pub tr
 
@@ -378,7 +447,6 @@ theorem Bytes.HasUsage_public
   := by
     grind [Bytes.HasUsage]
 
-noncomputable
 def Bytes.xxxLabel
   [GetLabel]
   (extract: Bytes → Option Bytes)
