DY/ALaCarte/Basic.lean
@@ -1,0 +1,519 @@
+namespace DY.ALaCarte
+/--
+  Compute the sum of `sizeOf` on the `t` contained by `Functor`.
+  This is needed to prove `Representable.sizeOf_eq`.
+-/
+class FunctorSizeOf (f: Type → Type) where
+  sizeOf {t: Type} [SizeOf t]: f t → Nat
+
+-- SubFunctor / SubFunctorTC is inspired by Coe / CoeTC
+-- Could be split in SubFunctor / LawfulSubFunctor to avoid dependency on FunctorSizeOf?
+class SubFunctor (f: Type → Type) (g: semiOutParam (Type → Type)) [FunctorSizeOf f] [semiOutParam (FunctorSizeOf g)] where
+  inj: {a: Type} → f a → g a
+  proj: {a: Type} → g a → Option (f a)
+  proj_inj {a: Type}:
+    ∀ x: f a, proj (inj x) = some x
+  inj_proj {a: Type}:
+    ∀ x: g a,
+    match proj x with
+    | some y => inj y = x
+    | none => True
+  sizeOf_inj {a: Type} [SizeOf a] (x: f a):
+    FunctorSizeOf.sizeOf (inj x) = FunctorSizeOf.sizeOf x
+
+-- Transitive Closure for SubFunctor
+-- Inspired by Coe / CoeTC
+class SubFunctorTC (f g: Type → Type) [FunctorSizeOf f] [FunctorSizeOf g] where
+  inj: {a: Type} → f a → g a
+  proj: {a: Type} → g a → Option (f a)
+  proj_inj {a: Type}:
+    ∀ x: f a, proj (inj x) = some x
+  inj_proj {a: Type}:
+    ∀ x: g a,
+    match proj x with
+    | some y => inj y = x
+    | none => True
+  sizeOf_inj {a: Type} [SizeOf a] (x: f a):
+    FunctorSizeOf.sizeOf (inj x) = FunctorSizeOf.sizeOf x
+
+instance (f: Type → Type) [FunctorSizeOf f]: SubFunctorTC f f where
+  inj x := x
+  proj x := x
+  proj_inj x := rfl
+  inj_proj x := by simp
+  sizeOf_inj x := by simp
+
+instance {f g h: Type → Type} [FunctorSizeOf f] [FunctorSizeOf g] [FunctorSizeOf h] [SubFunctor f g] [SubFunctorTC g h]: SubFunctorTC f h where
+  inj x := SubFunctorTC.inj (SubFunctor.inj (g := g) x)
+  proj x :=
+    match SubFunctorTC.proj (f := g) x with
+    | none => none
+    | some x' => SubFunctor.proj x'
+  proj_inj x := by grind [SubFunctorTC.proj_inj, SubFunctor.proj_inj]
+  inj_proj x := by grind [SubFunctorTC.inj_proj, SubFunctor.inj_proj]
+  sizeOf_inj x := by simp [SubFunctorTC.sizeOf_inj, SubFunctor.sizeOf_inj]
+
+structure Ctor where
+  Data: Type 0
+  nRec: Nat
+
+def Ctors (CtorId: Type) := CtorId -> Ctor
+
+structure FunctorRepr {CtorId} (ctors: Ctors CtorId) (a: Type) where
+  id: CtorId
+  data: (ctors id).Data
+  as: Vector a ((ctors id).nRec)
+
+noncomputable
+instance {CtorId} (ctors: Ctors CtorId): FunctorSizeOf (FunctorRepr ctors) where
+  sizeOf | {id := _, data := _, as} => (as.map sizeOf).sum
+
+-- Could be split in Representable / LawfulRepresentable to avoid dependency on FunctorSizeOf
+class Representable (f: Type → Type) [FunctorSizeOf f] where
+  CtorId: Type
+  ctors: Ctors CtorId
+  toRepr: {a: Type} → f a → FunctorRepr ctors a
+  fromRepr: {a: Type} → FunctorRepr ctors a → f a
+  from_to: {a: Type} → ∀ x: f a, fromRepr (toRepr x) = x
+  to_from: {a: Type} → ∀ x: FunctorRepr ctors a, toRepr (fromRepr x) = x
+  sizeOf_eq {a: Type} [SizeOf a]: ∀ x: f a, FunctorSizeOf.sizeOf x = FunctorSizeOf.sizeOf (toRepr x)
+
+structure BareContainer {CtorId} (ctors: Ctors CtorId) where
+  id: CtorId
+  data: (ctors id).Data
+  as: Array (BareContainer ctors)
+
+theorem Array.sizeOf_mem
+  {α: Type} [SizeOf α]
+  (arr: Array α) (x: α)
+  : x ∈ arr → sizeOf x < sizeOf arr
+  := by
+    cases arr
+    rename_i l
+    induction l
+    · simp
+    simp_all
+    grind
+
+def BareContainer.wf {CtorId} {ctors: Ctors CtorId} (x: BareContainer ctors): Prop :=
+  x.as.size = (ctors x.id).nRec ∧
+  ∀ y, y ∈ x.as → y.wf
+termination_by sizeOf x
+decreasing_by
+  have := Array.sizeOf_mem x.as y (by assumption)
+  cases x
+  simp_all
+  grind
+
+def Container {CtorId} (ctors: Ctors CtorId): Type :=
+  Subtype (BareContainer.wf (ctors := ctors))
+
+noncomputable
+instance {CtorId: Type} (ctors: Ctors CtorId) [SizeOf CtorId]: SizeOf (Container ctors) := inferInstanceAs (SizeOf (Subtype (BareContainer.wf (ctors := ctors))))
+
+abbrev ContainerFor (f: Type → Type) [FunctorSizeOf f] [Representable f] :=
+  Container (Representable.ctors (f := f))
+
+theorem Array.unattach_p
+  {a: Type u}
+  {p: a → Prop}
+  (arr: Array (Subtype p))
+  : ∀ x, x ∈ arr.unattach → p x
+  := by
+    simp_all [Array.unattach, -Array.map_subtype]
+
+theorem Array.attachWith_unattach
+  {a: Type u}
+  {p: a → Prop}
+  (arr: Array (Subtype p)) (h: ∀ x, x ∈ (Array.unattach arr) → p x)
+  : Array.attachWith (Array.unattach arr) p h = arr
+  := by
+    cases arr
+    rename_i l
+    simp only [Array.attachWith, Array.unattach]
+    simp only [List.unattach_toArray, List.mem_toArray] at h
+    induction l <;>
+    simp_all
+
+def Container.intoFunctor
+  {CtorId: Type} {ctors: Ctors CtorId}
+  (x: Container ctors)
+  : FunctorRepr ctors (Container ctors)
+  where
+    id := x.val.id
+    data := x.val.data
+    as := Vector.mk (x.val.as.attachWith BareContainer.wf (by
+      have := x.property
+      rewrite [BareContainer.wf] at this
+      simp_all
+    )) (by
+      have := x.property
+      rewrite [BareContainer.wf] at this
+      rewrite [Array.size_attachWith]
+      simp_all
+    )
+
+def Container.fromFunctor
+  {CtorId: Type} {ctors: Ctors CtorId}
+  (x: FunctorRepr ctors (Container ctors))
+  : Container ctors
+  := Subtype.mk {
+    id := x.id
+    data := x.data
+    as := x.as.toArray.unattach
+  } (by
+    rewrite [BareContainer.wf]
+    grind [Array.size_unattach, Array.unattach_p]
+  )
+
+def Container.intoFunctor_fromFunctor
+  {CtorId: Type} {ctors: Ctors CtorId}
+  (x: FunctorRepr ctors (Container ctors))
+  : Container.intoFunctor (Container.fromFunctor x) = x
+  := by
+    cases x; rename_i id data as
+    rewrite [Container.fromFunctor, Container.intoFunctor]
+    simp [Array.attachWith_unattach]
+
+def Container.fromFunctor_intoFunctor
+  {CtorId: Type} {ctors: Ctors CtorId}
+  (x: Container ctors)
+  : Container.fromFunctor (Container.intoFunctor x) = x
+  := by
+    cases x; rename_i x h_x
+    cases x; rename_i id data as
+    rewrite [Container.fromFunctor, Container.intoFunctor]
+    simp
+
+theorem List.map_sizeOf_attachWith
+  {α: Type} [SizeOf α]
+  (l : List α) (P : α → Prop) (H : ∀ x ∈ l, P x)
+  : (List.map sizeOf (l.attachWith P H)).sum ≤ sizeOf l
+  := by
+    induction l <;>
+    simp_all
+
+theorem Container.sizeOf_intoFunctor
+  {CtorId: Type} {ctors: Ctors CtorId}
+  (x: Container ctors)
+  : FunctorSizeOf.sizeOf (Container.intoFunctor x) < sizeOf x
+  := by
+    cases x; rename_i val property
+    cases val; rename_i id data as
+    cases as; rename_i l
+    rewrite [Subtype.mk.sizeOf_spec]
+    simp only [FunctorSizeOf.sizeOf, intoFunctor, List.attachWith_toArray, Vector.map_mk, List.map_toArray, Vector.sum_mk, List.sum_toArray, BareContainer.mk.sizeOf_spec, sizeOf_default, Nat.add_zero, Array.mk.sizeOf_spec]
+    refine Nat.lt_add_left 1 ?_
+    refine Nat.lt_add_left 1 ?_
+    refine Nat.lt_one_add_iff.mpr ?_
+    apply List.map_sizeOf_attachWith
+
+structure FunctorUnion {a: Type} (Functors: a → (Type → Type)) (t: Type) where
+  id: a
+  val: Functors id t
+
+structure FunctorUnion.CtorId {a: Type} (Functors: a → (Type → Type)) [∀ id, FunctorSizeOf (Functors id)] [∀ id, Representable (Functors id)] where
+  idHead: a
+  idTail: Representable.CtorId (Functors idHead)
+
+instance {a: Type} (Functors: a → (Type → Type)) [∀ id, FunctorSizeOf (Functors id)]: FunctorSizeOf (FunctorUnion Functors) where
+  sizeOf x :=
+    FunctorSizeOf.sizeOf x.val
+
+instance {a: Type} (Functors: a → (Type → Type)) [∀ id, FunctorSizeOf (Functors id)] [∀ id, Representable (Functors id)]: Representable (FunctorUnion Functors)
+  where
+    CtorId := FunctorUnion.CtorId Functors
+    ctors id :=
+      (Representable.ctors (f := Functors id.idHead)) id.idTail
+    toRepr x :=
+      let reprMid := Representable.toRepr (f := Functors x.id) x.val
+      { reprMid with
+        id := {
+          idHead := x.id,
+          idTail := reprMid.id
+        }
+      }
+    fromRepr repr :=
+      {
+        id := repr.id.idHead
+        val := Representable.fromRepr (f := Functors repr.id.idHead) { repr with id := repr.id.idTail }
+      }
+    from_to := by
+      intro a x
+      simp_all [Representable.from_to (f := Functors x.id) x.val]
+    to_from := by
+      intro a repr
+      have := Representable.to_from (f := Functors repr.id.idHead) { repr with id := repr.id.idTail }
+      cases repr
+      simp_all
+      grind
+    sizeOf_eq x := by
+      simp only [FunctorSizeOf.sizeOf]
+      have := Representable.sizeOf_eq x.val
+      revert this
+      generalize (Representable.toRepr x.val) = y
+      cases y
+      simp [FunctorSizeOf.sizeOf]
+
+instance {a: Type} [DecidableEq a] (Functors: a → (Type → Type)) [∀ id, FunctorSizeOf (Functors id)] (id: a): SubFunctor (Functors id) (FunctorUnion Functors) where
+  inj x := {
+    id := id
+    val := x
+  }
+  proj x :=
+    if h: x.id = id then
+      some (h ▸ x.val)
+    else
+      none
+  proj_inj x := by grind
+  inj_proj x := by cases x; grind
+  sizeOf_inj x := by simp [FunctorSizeOf.sizeOf]
+
+def Container.pack (f: Type → Type) {g: Type → Type} [FunctorSizeOf f] [FunctorSizeOf g] [SubFunctorTC f g] [Representable g] (x: f (ContainerFor g)): (ContainerFor g) :=
+  Container.fromFunctor (
+    Representable.toRepr (
+      SubFunctorTC.inj x
+    )
+  )
+
+def Container.view (f: Type → Type) {g: Type → Type} [FunctorSizeOf f] [FunctorSizeOf g] [SubFunctorTC f g] [Representable g] (x: ContainerFor g): Option (f (ContainerFor g)) :=
+  SubFunctorTC.proj (
+    Representable.fromRepr (
+      Container.intoFunctor x
+    )
+  )
+
+theorem Container.view_pack
+  (f: Type → Type) {g: Type → Type}
+  [FunctorSizeOf f] [FunctorSizeOf g]
+  [SubFunctorTC f g] [Representable g]
+  (x: f (ContainerFor g))
+  : view f (pack f x) = some x
+  := by
+    unfold view pack
+    simp [Container.intoFunctor_fromFunctor, Representable.from_to, SubFunctorTC.proj_inj]
+
+theorem Container.pack_view
+  (f: Type → Type) {g: Type → Type}
+  [FunctorSizeOf f] [FunctorSizeOf g]
+  [SubFunctorTC f g] [Representable g]
+  (x: ContainerFor g)
+  : match view f x with
+    | none => True
+    | some y => pack f y = x
+  := by
+    unfold view pack
+    split
+    · trivial
+    · have := SubFunctorTC.inj_proj (f := f) (Representable.fromRepr x.intoFunctor)
+      have := Representable.to_from x.intoFunctor
+      have := Container.fromFunctor_intoFunctor x
+      simp_all
+
+def Container.PartialFunDep
+  (f: Type → Type) {g: Type → Type} [FunctorSizeOf f] [FunctorSizeOf g] [Representable g] [SubFunctorTC f g]
+  (motive: ContainerFor g → Sort u)
+  :=
+  (∀ x: f (ContainerFor g), (∀ y: ContainerFor g, (h: sizeOf y ≤ FunctorSizeOf.sizeOf x := by simp_all +arith [DY.ALaCarte.FunctorSizeOf.sizeOf]) → motive y) → motive (pack f x))
+
+-- This one does not require the typeclass instance [SubFunctorTC f g]
+def Container.PartialFun
+  (f: Type → Type) (g: Type → Type) [FunctorSizeOf f] [FunctorSizeOf g] [Representable g]
+  (a: Type)
+  :=
+  ∀ x: f (ContainerFor g), (∀ y: ContainerFor g, (h: sizeOf y ≤ FunctorSizeOf.sizeOf x := by simp_all +arith [DY.ALaCarte.FunctorSizeOf.sizeOf]) → a) → a
+
+def Container.rec
+  {f: Type → Type} [FunctorSizeOf f] [Representable f]
+  {motive: ContainerFor f → Sort u}
+  (pf: Container.PartialFunDep f motive)
+  (x: ContainerFor f)
+    : motive x := by
+  have := pf (Representable.fromRepr (Container.intoFunctor x)) (fun y h => Container.rec pf y)
+  simp only [pack, SubFunctorTC.inj, Representable.to_from, Container.fromFunctor_intoFunctor] at this
+  exact this
+termination_by x
+decreasing_by
+  have := Representable.sizeOf_eq (Representable.fromRepr (Container.intoFunctor x))
+  have := Representable.to_from (Container.intoFunctor x)
+  have := Container.sizeOf_intoFunctor x
+  grind
+
+class SubPartialFun
+  {f g h: Type → Type}
+  [FunctorSizeOf f] [FunctorSizeOf g] [FunctorSizeOf h]
+  [Representable h]
+  [SubFunctor f g]
+  {a: Type}
+  (f1: Container.PartialFun f h a)
+  (f2: semiOutParam (Container.PartialFun g h a))
+    where
+  pf (f1 f2): ∀ x rec, f1 x rec = f2 (SubFunctor.inj x) (fun y h => rec y (by simp_all [SubFunctor.sizeOf_inj x]))
+
+class SubPartialFunTC
+  {f g h: Type → Type}
+  [FunctorSizeOf f] [FunctorSizeOf g] [FunctorSizeOf h]
+  [Representable h]
+  [SubFunctorTC f g]
+  {a: Type}
+  (f1: Container.PartialFun f h a)
+  (f2: Container.PartialFun g h a)
+    where
+  pf (f1 f2): ∀ x rec, f1 x rec = f2 (SubFunctorTC.inj x) (fun y h => rec y (by simp_all [SubFunctorTC.sizeOf_inj x]))
+
+instance {f: Type → Type} [FunctorSizeOf f] [Representable f] {a: Type} (f: Container.PartialFun f f a): SubPartialFunTC f f where
+  pf := by
+    simp [SubFunctorTC.inj]
+
+instance
+  {f g h i: Type → Type}
+  [FunctorSizeOf f] [FunctorSizeOf g] [FunctorSizeOf h] [FunctorSizeOf i]
+  [Representable i]
+  [SubFunctor f g]
+  [SubFunctorTC g h]
+  {a: Type}
+  (f1: Container.PartialFun f i a)
+  (f2: Container.PartialFun g i a)
+  (f3: Container.PartialFun h i a)
+  [SubPartialFun f1 f2]
+  [SubPartialFunTC f2 f3]
+  : SubPartialFunTC f1 f3
+  where
+    pf := by
+      intro x rec
+      simp [SubFunctorTC.inj]
+      rewrite [← SubPartialFunTC.pf f2 f3 (SubFunctor.inj x) (fun y h => rec y (by grind [SubFunctor.sizeOf_inj]))]
+      rewrite [← SubPartialFun.pf f1 f2 x (fun y h => rec y (by grind))]
+      rfl
+
+theorem Container.rec_eq
+  {f: Type → Type} {g: Type → Type} [FunctorSizeOf f] [FunctorSizeOf g] [SubFunctorTC f g] [Representable g]
+  {a: Type}
+  (partialFun: Container.PartialFun f g a)
+  (totalFun: Container.PartialFun g g a)
+  [SubPartialFunTC partialFun totalFun]
+  (x: f (ContainerFor g))
+  : (pack f x).rec totalFun = partialFun x (fun y _ => y.rec totalFun)
+  := by
+    conv => lhs; unfold Container.rec pack
+    simp only [eq_mp_eq_cast, cast_eq]
+    rewrite [Container.intoFunctor_fromFunctor]
+    rewrite [Representable.from_to]
+    rewrite [<- SubPartialFunTC.pf partialFun totalFun x (fun y h => rec totalFun y)]
+    grind
+
+def Container.PartialFun.combine
+  {t: Type} [DecidableEq t]
+  {functors: t → Type → Type} [∀ id, FunctorSizeOf (functors id)]
+  {g: Type → Type} [FunctorSizeOf g] [Representable g]
+  {a: Type}
+  (funs: (id: t) → Container.PartialFun (functors id) g a)
+  : Container.PartialFun (FunctorUnion functors) g a
+  := fun {id, val} rec =>
+    funs id val (fun y h => rec y h)
+
+def Container.PartialFunDep.combine
+  {t: Type} [DecidableEq t]
+  {functors: t → Type → Type} [∀ id, FunctorSizeOf (functors id)]
+  {g: Type → Type} [FunctorSizeOf g] [Representable g]
+  [SubFunctorTC (FunctorUnion functors) g]
+  {motive: ContainerFor g → Sort u}
+  (funs: (id: t) → Container.PartialFunDep (functors id) motive)
+  : Container.PartialFunDep (FunctorUnion functors) motive
+  := fun {id, val} rec =>
+    funs id val (fun y h => rec y h)
+
+instance
+  {t: Type} [DecidableEq t]
+  {functors: t → Type → Type} [∀ id, FunctorSizeOf (functors id)]
+  {g: Type → Type} [FunctorSizeOf g] [Representable g]
+  {a: Type}
+  (funs: (id: t) → Container.PartialFun (functors id) g a)
+  (id: t)
+  : SubPartialFun (funs id) (Container.PartialFun.combine funs)
+  where
+    pf x rec := by
+      simp [Container.PartialFun.combine]
+
+def Container.PartialProof1
+  {f g: Type → Type} [FunctorSizeOf f] [FunctorSizeOf g] [Representable g]
+  {a: Type}
+  (fn: Container.PartialFun f g a)
+  (rec: ContainerFor g → a)
+  (p: a → Prop)
+  : Prop
+  := ∀ x: f (ContainerFor g), (∀ y: ContainerFor g, sizeOf y ≤ FunctorSizeOf.sizeOf x → p (rec y)) → p (fn x (fun y _ => rec y))
+
+theorem Container.PartialProof1.into
+  {f: Type → Type} [FunctorSizeOf f] [Representable f]
+  {a: Type}
+  {fn: Container.PartialFun f f a}
+  {p: a → Prop}
+  (pf: Container.PartialProof1 fn (Container.rec fn) p)
+  : Container.PartialFunDep f (fun x => p (x.rec fn))
+  := by
+    unfold Container.PartialFunDep autoParam
+    intro x rec
+    unfold Container.rec pack
+    simp only [SubFunctorTC.inj]
+    rewrite [Container.intoFunctor_fromFunctor]
+    rewrite [Representable.from_to]
+    exact pf x rec
+
+def Container.PartialProof1.combine
+  {t: Type} [DecidableEq t]
+  {functors: t → Type → Type} [∀ id, FunctorSizeOf (functors id)]
+  {g: Type → Type} [FunctorSizeOf g] [Representable g]
+  {a: Type}
+  {rec: ContainerFor g → a}
+  {p: a → Prop}
+  {funs: (id: t) → Container.PartialFun (functors id) g a}
+  (pfs: (id: t) → Container.PartialProof1 (funs id) rec p)
+  : Container.PartialProof1 (Container.PartialFun.combine funs) rec p
+  := fun {id, val} rec =>
+    pfs id val (fun y h => rec y h)
+
+def Container.PartialProof2
+  {f g: Type → Type} [FunctorSizeOf f] [FunctorSizeOf g] [Representable g]
+  {a b: Type}
+  (fn1: Container.PartialFun f g a)
+  (fn2: Container.PartialFun f g b)
+  (rec1: ContainerFor g → a)
+  (rec2: ContainerFor g → b)
+  (p: a × b → Prop)
+  : Prop
+  := ∀ x: f (ContainerFor g), (∀ y: ContainerFor g, sizeOf y ≤ FunctorSizeOf.sizeOf x → p (rec1 y, rec2 y)) → p (fn1 x (fun y _ => rec1 y), fn2 x (fun y _ => rec2 y))
+
+theorem Container.PartialProof2.into
+  {f: Type → Type} [FunctorSizeOf f] [Representable f]
+  {a b: Type}
+  {fn1: Container.PartialFun f f a}
+  {fn2: Container.PartialFun f f b}
+  {p: a × b → Prop}
+  (pf: Container.PartialProof2 fn1 fn2 (Container.rec fn1) (Container.rec fn2) p)
+  : Container.PartialFunDep f (fun x => p (x.rec fn1, x.rec fn2))
+  := by
+    unfold Container.PartialFunDep autoParam
+    intro x rec
+    unfold Container.rec pack
+    simp only [SubFunctorTC.inj]
+    rewrite [Container.intoFunctor_fromFunctor]
+    rewrite [Representable.from_to]
+    exact pf x rec
+
+def Container.PartialProof2.combine
+  {t: Type} [DecidableEq t]
+  {functors: t → Type → Type} [∀ id, FunctorSizeOf (functors id)]
+  {g: Type → Type} [FunctorSizeOf g] [Representable g]
+  {a b: Type}
+  {rec1: ContainerFor g → a}
+  {rec2: ContainerFor g → b}
+  {p: a × b → Prop}
+  {funs1: (id: t) → Container.PartialFun (functors id) g a}
+  {funs2: (id: t) → Container.PartialFun (functors id) g b}
+  (pfs: (id: t) → Container.PartialProof2 (funs1 id) (funs2 id) rec1 rec2 p)
+  : Container.PartialProof2 (Container.PartialFun.combine funs1) (Container.PartialFun.combine funs2) rec1 rec2 p
+  := fun {id, val} rec =>
+    pfs id val (fun y h => rec y h)
+
+end DY.ALaCarte
